cleaned

semantics/algorithms.v
@@ -4,63 +4,54 @@ From Coq Require Import Bool.Bool Init.Nat Arith.Arith Arith.EqNat
 Require Export Coq.Strings.String.
 From mathcomp Require Import ssreflect ssrfun ssrbool eqtype seq.
 From Semantics Require Export semantics lemmas_0.
+
 (*relation determining what variables are read from when evaluating exp e
  *)
-(*N, V are irrespective as they'll
-determine the values read, not the variables, just put them there for eeval to typecheck*)
 Inductive rd: exp -> warvars -> Prop :=
     RD: forall {e: exp} {N: nvmem} {V: vmem} {rs: readobs} {v: value},
       eeval N V e rs v -> rd e (readobs_wvs rs).
 
 
-
+(*the following relations are described in more detail in the technical appendix of 'Towards a Formal Foundation'*)
 Inductive WAR_ins: warvars -> warvars -> warvars -> instruction -> warvars -> warvars -> Prop :=
 WAR_Skip: forall(N W R: warvars),
     WAR_ins N W R skip W R
-| WAR_Vol: forall(N W R Re: warvars) (x: smallvar) (e: exp), (*rule for writing to volatile variables: does not change written set or check checkpoint*)
-             (rd e Re) -> (*extra premise checking that Re is the list of values read when e is evaluated*)
-             isV x -> (*x is volatile*)
-             (inl x) \notin W -> (*ensuring parameters are well formed*)
+| WAR_Vol: forall(N W R Re: warvars) (x: smallvar) (e: exp),
+    (rd e Re) -> 
+             isV x -> 
+             (inl x) \notin W -> 
              WAR_ins N W R (asgn_sv x e) W (Re ++ R)
 | WAR_NoRd: forall(N W R Re: warvars)
              (x: smallvar) (e: exp),
-             isNV x -> (*checking x is nonvolatile*)
-             (rd e Re) -> (*extra premise checking that Re is the list of values read when e is evaluated*)
+             isNV x -> 
+             (rd e Re) -> 
              not((inl x) \in (Re ++ R)) 
              -> WAR_ins N W R (asgn_sv x e) ((inl x)::W) (Re ++ R)
 | WAR_Checkpointed: forall(N W R Re: warvars)
              (x: smallvar) (e: exp),
-             (rd e Re) -> (*extra premise checking that Re is the list of values read when e is evaluated*)
-             isNV x -> (*checking x is nonvolatile*)
+             (rd e Re) -> 
+             isNV x -> 
              (inl x) \in (Re ++ R) ->
              not((inl x) \in W) ->
              ((inl x) \in N) ->
              WAR_ins N W R (asgn_sv x e) ((inl x)::W) (Re ++ R)
 | WAR_WT: forall(N W R Re: warvars)
              (x: smallvar) (e: exp),
-             (rd e Re) -> (*extra premise checking that Re is the list of values read when e is evaluated*)
+             (rd e Re) -> 
              (inl x) \in (Re ++ R) ->
                          ((inl x) \in W) ->
-             isNV x -> (*checking x is nonvolatile*)
+             isNV x -> 
              WAR_ins N W R (asgn_sv x e) ((inl x) ::W) (Re ++ R)
-(*no restrictions on the parameter W,
- if make W really big, never enter the checkpointed case
- and check N for anything
- concern w regard to lemma 13 which allows for
- an arbitrary W to be chosen*)
 | WAR_NoRd_Arr: forall(N W R Re Rindex: warvars)
                  (a: array) (e index: exp),
-    (rd e Re) -> (*extra premise checking that Re is the list of values read when e is evaluated*)
-    (rd index Rindex) -> (*extra premise checking that Rindex is the list of values read when index is evaluated*)
-    not(intersect (generate_locs a) (Re ++ Rindex ++ R)) -> (*would be easier
-                                                        if you had intersection here
-                                                       ~subseq is weak *)
-    WAR_ins N W R (asgn_arr a index e) ((generate_locs a) ++ W) (Re ++ Rindex ++ R) (*written set is modified but
-                                                                        don't need to check if a is NV cuz all arrays are*)
+    (rd e Re) -> 
+    (rd index Rindex) -> 
+    not(intersect (generate_locs a) (Re ++ Rindex ++ R)) ->
+    WAR_ins N W R (asgn_arr a index e) ((generate_locs a) ++ W) (Re ++ Rindex ++ R)
 | WAR_Checkpointed_Arr: forall(N W R Re Rindex: warvars)
                  (a: array) (e index: exp),
-    (rd e Re) -> (*extra premise checking that Re is the list of values read when e is evaluated*)
-    (rd index Rindex) -> (*extra premise checking that Rindex is the list of values read when index is evaluated*)
+    (rd e Re) -> 
+    (rd index Rindex) -> 
     (subseq (generate_locs a) (Re ++ Rindex ++ R)) ->
     (subseq (generate_locs a)  N) ->
     WAR_ins N W R (asgn_arr a index e) ((generate_locs a) ++ W) (Re ++ Rindex ++ R)
@@ -80,51 +71,52 @@ Inductive WARok: warvars -> warvars -> warvars -> command -> Prop:=
  | WAR_If: forall(N W R Re: warvars)
             (e: exp)
             (c1 c2: command),
-     (rd e Re) -> (*extra premise checking that Re is the list of values read when e is evaluated*)
+     (rd e Re) -> 
      WARok N W (Re ++ R) c1 ->
      WARok N W (Re ++ R) c2 ->
      WARok N W R (TEST e THEN c1 ELSE c2)
 .
 
+(*relations modeling the DINO algorithm*)
 Inductive DINO_ins: warvars -> warvars -> warvars -> instruction
                 -> warvars -> warvars -> warvars -> Prop:=
   D_WAR_Skip: forall(N W R: warvars),
     DINO_ins N W R skip N W R
-| D_WAR_Vol: forall(N W R Re: warvars) (x: smallvar) (e: exp), (*rule for writing to volatile variables: does not change written set or check checkpoint*)
-             (rd e Re) -> (*extra premise checking that Re is the list of values read when e is evaluated*)
-             isV x -> (*x is volatile*)
+| D_WAR_Vol: forall(N W R Re: warvars) (x: smallvar) (e: exp),
+    (rd e Re) -> 
+             isV x -> 
              (inl x) \notin W ->
              DINO_ins N W R (asgn_sv x e) N W (Re ++ R)
 | D_WAR_Written: forall(N W R Re: warvars)
                   (x: smallvar) (e: exp),
-             (rd e Re) -> (*extra premise checking that Re is the list of values read when e is evaluated*)
-             isNV x -> (*checking x is nonvolatile*)
+             (rd e Re) -> 
+             isNV x -> 
              not((inl x) \in (Re ++ R))
              -> DINO_ins N W R (asgn_sv x e) N ((inl x)::W) (Re ++ R)
-| D_WAR_CP_Asgn: forall(N W R Re: warvars) (x: smallvar) (e: exp), (*Changed name to avoid duplication w D_WAR_CP below*)
-             (rd e Re) -> (*extra premise checking that Re is the list of values read when e is evaluated*)
-             isNV x -> (*checking x is nonvolatile*)
+| D_WAR_CP_Asgn: forall(N W R Re: warvars) (x: smallvar) (e: exp),
+    (rd e Re) -> 
+             isNV x -> 
              (inl x) \in (Re ++ R) ->
              not((inl x) \in W) ->
              DINO_ins N W R (asgn_sv x e)
                   ((inl x)::N) ((inl x)::W) (Re ++ R)
 | D_WAR_WtDom: forall(N W R Re: warvars) 
              (x: smallvar) (e: exp),
-             (rd e Re) -> (*extra premise checking that Re is the list of values read when e is evaluated*)
+             (rd e Re) -> 
              (inl x) \in (Re ++ R) ->
                          ((inl x) \in W) ->
                          isNV x ->
              DINO_ins N W R (asgn_sv x e) N ((inl x) ::W) (Re ++ R)
 | D_WAR_Wt_Arr: forall(N W R Re Rindex: warvars)
                  (a: array) (e index: exp),
-    (rd e Re) -> (*extra premise checking that Re is the list of values read when e is evaluated*)
-    (rd index Rindex) -> (*extra premise checking that Rindex is the list of values read when index is evaluated*)
+    (rd e Re) -> 
+    (rd index Rindex) -> 
     not(intersect (generate_locs a) (Re ++ Rindex ++ R)) ->
     DINO_ins N W R (asgn_arr a index e) N ((generate_locs a) ++ W) (Re ++ Rindex ++ R)
 | D_WAR_CP_Arr: forall(N W R Re Rindex: warvars)
                  (a: array) (e index: exp), 
-    (rd e Re) -> (*extra premise checking that Re is the list of values read when e is evaluated*)
-    (rd index Rindex) -> (*extra premise checking that Rindex is the list of values read when index is evaluated*)
+    (rd e Re) -> 
+    (rd index Rindex) -> 
                 subseq (generate_locs a) (Re ++ Rindex ++ R) ->
                  DINO_ins N W R (asgn_arr a index e)
              ((generate_locs a) ++ N) ((generate_locs a)++ W) (Re ++ Rindex ++ R)
@@ -141,7 +133,7 @@ Inductive DINO: warvars -> warvars -> warvars -> command
     DINO N' W' R' c c' N''  ->
     DINO N W R (l;;c) (l;;c') N''
 | D_WAR_If: forall(N N1 N2 W R Re: warvars) (c1 c1' c2 c2': command) (e: exp),
-             (rd e Re) -> (*extra premise checking that Re is the list of values read when e is evaluated*)
+             (rd e Re) -> 
      DINO N W (Re ++ R) c1 c1' N1 ->
      DINO N W (Re ++ R) c2 c2' N2 ->
      DINO N W R (TEST e THEN c1 ELSE c2) (TEST e THEN c1' ELSE c2') (N1 ++ N2)
