semantics/programs.v
@@ -14,47 +14,7 @@ Implicit Types x: smallvar.
 Open Scope type_scope.
 (************* program traces*****************)
 
-(*trace helpers*)
-
-(*Notes:*)
-(*do I keep track of volatile writes as well...I don't think so
- cuz the writes don't last and they all have to be checkpointed anyways*)
-(*concern:*)
-(*actually there's no reason for us to be checkpointing volatiles that are
- written to before they're ever read from along any path*)
-(*at first inspection it doesn't seem like it would be all that hard to keep track of this
- since we're already doing MFstWt for novolatiles.*)
-
-(*concern: cconf and context are functionally the same but cconf has an annoying constructor
- which can't be coerced bc context exists, consider combining into one type?*)
-
-(*The trace type contains
-1. starting configuration
-2. ending configuration
-3. execution observations
-4. a list of warvars which have been written to
-5. a list of warvars which have been read from
-6. a list of warvars which have been written to before they have been read from
- *)
-(*Ordering: start -> end -> observations -> the_write_stuff*)
-(*steps to termination, accumulates write data*)
-
 (*continuous traces*)
-
-Inductive trace_c: context -> context -> obseq -> the_write_stuff -> Prop :=
-  CTrace_Empty: forall(C: context),
-                 trace_c C C [::] ([::], [::], [::])
-  | CTrace_Single: forall {C1 C2: context} {O: obseq} {W: the_write_stuff},
-      cceval_w C1 O C2 W ->
-      trace_c C1 C2 O W
-| CTrace_App: forall{C1 C2 Cmid: context} {O1 O2: obseq}
-               {W1 W2: the_write_stuff},
-    trace_c C1 Cmid O1 W1 -> (*steps first section*)
-    O1 <> [::] -> (* forces empty step to use other constructors*)
-    O2 <> [::]  ->
-    trace_c Cmid C2 O2 W2 -> (*steps rest of program*)
-    trace_c C1 C2 (O1 ++ O2) (append_write W1 W2).
-
 Inductive trace_cs: context -> context -> obseq -> the_write_stuff -> Prop :=
   CsTrace_Empty: forall(C: context),
                  trace_cs C C [::] ([::], [::], [::])
@@ -63,99 +23,12 @@ Inductive trace_cs: context -> context -> obseq -> the_write_stuff -> Prop :=
       trace_cs C1 C2 O W
 | CsTrace_Cons: forall{C1 Cmid C2: context} {O1 O2: obseq}
                {W1 W2: the_write_stuff},
-    trace_cs Cmid C2 O2 W2 -> (*steps last section*)
-    O2 <> [::] -> (* forces empty step to use other constructors*)
+    trace_cs Cmid C2 O2 W2 -> 
+    O2 <> [::] -> 
     cceval_w C1 O1 Cmid W1 ->
     trace_cs C1 C2 (O1 ++ O2) (append_write W1 W2).
 
-
-
-(*Inductive trace_c1: context -> context -> obseq -> the_write_stuff -> Prop :=
-  CTrace_Empty: forall(C: context),
-                 trace_c C C [::] ([::], [::], [::])
-  | CTrace_Cons: forall {C1 Cmid C2: context} {O O2: obseq} {W W2: the_write_stuff},
-      trace_c Cmid C2 O2 W2 ->
-      cceval_w C1 O C2 W ->
-      trace_c C1 C2 (O ++ O2) (append_write W W2).*)
-
-(*induct over Os instead*)
-
-(*App makes for easy subtraces by allowing command in C2 not to be skip*)
-(*never actually need to append traces now that I have the write datatype
- consider a simpler type?*)
-
-Print trace_c_ind.
-
-
-
-
-(*if you need the empty cat thing come back here*)
-(*Lemma empty_trace: forall{C1 C2: context} {O: obseq} {W: the_write_stuff},
-    trace_c C1 C2 O W -> O = [::] -> C1 = C2 /\ W = emptysets.
-Proof. intros. inversion H; subst.
-       + split; reflexivity.
-       + inversion H1.
-       + 
-         exfalso.
- move / nilP : H7 => H7.
-         unfold nilp in H7.
-         apply (elimT eqP) in H7.
-         rewrite (size_cat O1 O2) in H7.
-         move / eqP : H7.
-         rewrite addn_eq0.
-         apply / andb_true_iff => H10.
-         destruct H10.
-         by move / nilP / H2 : H0.*)
-
-(*use trace_steps, cceval_steps, cceval_steps ins*)
-
-
-Program Definition trace_append {C1 Cmid C2: context }
-                  {O1 O2: obseq}
-                  {W1 W2: the_write_stuff}
-                  (T1: trace_c C1 Cmid O1 W1)
-                  (T2: trace_c Cmid C2 O2 W2) : trace_c C1 C2 (O1 ++ O2) (append_write W1 W2)
-  :=
-  match O1, O2 with
-    [::], [::] => T1 (*C1 = Cmid = C2*)
-  | [::], _ => T2 (*C1 = Cmid*)
-  | _, [::] => T1 (**)
-  | (x::xs), (y::ys) => CTrace_App T1 _ _ T2 end.
-
-
-
 (*intermittent traces*)
- (*the same as trace_c bar types as differences between
-  intermittent and continuous execution have been implemented in evals
-Inductive trace_i : iconf -> iconf -> obseq -> the_write_stuff -> Prop :=
-iTrace_Empty: forall{C: iconf},
-                 trace_i C C [::] ([::], [::], [::])
-|iTrace_Single: forall{C1 C2: iconf} {O: obseq} {W: the_write_stuff},
-                  iceval_w C1 O C2 W -> (*command in C2 is skip by def single_com, iceval_w*)
-                  trace_i C1 C2 O W
-| iTrace_App: forall{C1 C2 Cmid: iconf} {O1 O2: obseq}
-         {W1 W2: the_write_stuff},
-    trace_i C1 Cmid O1 W1 -> (*steps first section*)
-    trace_i Cmid C2 O2 W2 -> (*steps rest of program*)
-    O1 <> [::] -> (* forces empty step to use other constructors*)
-    O2 <> [::]  ->
-    trace_i C1 C2 (O1 ++ O2) (append_write W1 W2).
-(*could force the CPs to be well intialized here as well by controlling context in itrace
- Single and in 1st arg to itrace _app*)
-
-Inductive trace_is : iconf -> iconf -> obseq -> the_write_stuff -> Prop :=
-isTrace_Empty: forall{C: iconf},
-                 trace_is C C [::] ([::], [::], [::])
-|isTrace_Single: forall{C1 C2: iconf} {O: obseq} {W: the_write_stuff},
-                  iceval_w C1 O C2 W -> (*command in C2 is skip by def single_com, iceval_w*)
-                  trace_is C1 C2 O W
-| isTrace_Cons: forall{C1 C2 Cmid: iconf} {O1 O2: obseq}
-         {W1 W2: the_write_stuff},
-    iceval_w C1 O1 Cmid W1 -> (*steps first section*)
-    trace_is Cmid C2 O2 W2 -> (*steps rest of program*)
-    O2 <> [::]  ->
-    trace_is C1 C2 (O1 ++ O2) (append_write W1 W2).*)
-
 Inductive trace_i1: iconf -> iconf -> obseq -> the_write_stuff -> Prop :=
   iTrace_Cont: forall(N0: nvmem) (V0: vmem) (c0: command)
     {N N1: nvmem} {V V1: vmem} {c c1: command}
@@ -183,83 +56,10 @@ Inductive trace_i1: iconf -> iconf -> obseq -> the_write_stuff -> Prop :=
                                                                                                checkpointed section*)
                         -> checkpoint \notin O1
                         -> trace_i1 (((restrict Nmid w Hw), Vmid, crem), Nmid, Vmid, crem)
-                                   ((Nc1, Vc1, cc1), Nend, Vend, cend) O2 W2
+                                   ((Nc1, Vc1, cc1), Nend, Vend, cend) O2 W2 (*remainder of trace*)
                         -> trace_i1 ((Nc0, Vc0, cc0), N0, V0, c0)
                                    ((Nc1, Vc1, cc1), Nend, Vend, cend)
                                    (O1 ++ [::checkpoint] ++ O2)
                                    (append_write W1 W2).
 
-
-(*relations between continuous and intermittent memory*)
-
-
-(*Definition 4*)
-(*concern: not yet clear to me why we need the vmem parameter; pending further inspection of
- proofs*)
-(*concern: liberal use of intensional equality with nvmem*)
-(*N0, V0 is starting state for both (maybe just continuous actually) executions
- N1, V1 and Ncomp are middle states of intermittent, continuous respectively
- V1 isn't used anywhere it's just to fill out the type
- N2, V2 is final state for intermittent, once again solely to fill out the type*)
-
-Inductive same_pt: nvmem -> vmem -> command -> command -> nvmem -> nvmem -> Prop :=
-same_mem: forall {N0 N1 Ncomp N2: nvmem}
-                  {V0 V1 V2: vmem}
-                  {c0 c1 crem: command}
-                  {W1 W2: the_write_stuff}
-                  {O1 O2: obseq}
-                  (T1: trace_c (N0, V0, c0) (N1, V1, c1) O1 W1)
-                  (T2: trace_c (N1, V1, c1) (N2, V2, crem) O2 W2),
-    crem = skip \/ (exists(w: warvars) (crem2: command), crem = ((incheckpoint w);;crem2)) ->
-                  subseq (getdomain Ncomp) (getdomain Ncomp) (*start here fix this*) 
-                  -> (checkpoint \notin O1)
-                  -> (checkpoint \notin O2) (*checks checkpoint T2 ends on is nearest checkpoint*)
-                 -> (forall(l: loc),
-                      not((getmap N1) l = (getmap Ncomp) l)
-                      -> ((l \in (getwt W2)) /\ (l \in (getfstwt (append_write W1 W2))) /\ not (l \in (getwt W1))))
-                  -> same_pt N0 V0 c0 c1 N1(*V1*) Ncomp.
-(*Definition 5*)
-(*Nc0 is starting nvm for cont
-Ni0 is starting nvm for intermittent
- N1 V1 is middle state for intermittent
-N, V, c is checkpoint at middle state of intermittent
- Nend, Vend is final state for intermittent, not used, solely to fill out the type
- V1 isn't used anywhere it's just to fill out the type
- N2, V2 is final state for intermittent, once again solely to fill out the type*)
-Inductive current_init_pt: nvmem -> vmem -> command -> nvmem -> nvmem -> nvmem -> Prop:=
-  valid_mem: forall {N Ni0 N1 Nc0 Nend: nvmem}
-                  {V V1 Vend: vmem}
-                  {c crem: command}
-                  {W : the_write_stuff}
-                  {O: obseq}
-                  {w: warvars}
-                  (T: trace_c (Ni0, V, c) (Nend, Vend, crem) O W),
-    crem = skip \/ (exists(w: warvars) (crem2: command), crem = ((incheckpoint w);;crem2)) ->
-                 subseq (getdomain Nc0) (getdomain N1) (*start here
-                                                        fix this*)
-                  -> subset_nvm N Nc0
-                  -> (checkpoint \notin O) (*checks checkpoint T ends on is nearest checkpoint*)
-                 -> (forall(l: loc),
-                      not((getmap N1) l = (getmap Nc0) l)
-                      -> (l \in (getfstwt W)) \/ (l \in (getdomain N)))
-                 -> current_init_pt N V c Ni0 N1 (*V1*) Nc0.
-(*Definition 6*)
-(*concern: Typo in paper, N0, V0 is left out of invocation of Def 4*)
-(*(N0, V0, c0) is checkpoint state at time c1
-N1 V c is intermittent state
-N2 V c is continuous state starting from same state as checkpoint
-concern: using context instead of cconf
- *)
-(*took out equality premises and built them into the types*)
-Check same_pt.
-Inductive same_config: nvmem -> iconf -> context -> Prop :=
-  SameConfig: forall(Nstart N0 N1 N2: nvmem)
-                (V0 V: vmem)
-                (c0 c: command),
-    subset_nvm N0 Nstart ->
-                same_pt Nstart V0 c0 c N1 (*V*) N2 -> (*nvms are extensionally the same by same_pt
-                                          vms and cs are intensionally the same by types*)
-                same_config Nstart ((N0, V0, c0), N1, V, c) (N2, V, c).
-
-
-Close Scope type_scope.
+Definition end_com c := c = Ins skip \/ exists(crem: command)(w: warvars), c= (incheckpoint w);; crem.
