semantics/proofs.v
@@ -1,0 +1,698 @@
+Set Warnings "-notation-overridden,-parsing".
+From Coq Require Import Bool.Bool Init.Nat Arith.Arith Arith.EqNat
+     Init.Datatypes Strings.String Program Logic.FunctionalExtensionality.
+Require Export Coq.Strings.String.
+From mathcomp Require Import ssreflect ssrfun ssrbool eqtype seq fintype ssrnat ssrfun.
+From TLC Require Import LibTactics LibLogic.
+From Semantics Require Export programs semantics algorithms lemmas_1
+     lemmas_0 proofs_0 proofs_w. 
+Implicit Types N: nvmem. Implicit Types V: vmem.
+Implicit Types O: obseq.
+Implicit Types c: command.
+Implicit Types W: the_write_stuff.
+Implicit Types x: smallvar.
+
+(*The exciting proofs are at the bottom. More important lemmas are briefly commented.*)
+
+(*Invariants*)
+
+(*My memory invariant. I like it because it is minimalistic, yet sufficient (along with its weaker version, which differs only in the ommision of the requirement that end_com c2) to prove the final correctness result. Further, it is preserved after arbitrary reboot, provided that the DINO checkpointing scheme is followed, which facillitates reasoning about intermittent execution.
+ Also, it is an equivalence relation, as proved below.*)
+Inductive all_diff_in_fw: nvmem -> vmem -> command -> nvmem -> Prop :=
+  Diff_in_FW: forall{N1 V1 c1 N2 V2 c2 N1c O W} (T: trace_cs (N1, V1, c1) (N2, V2, c2) O W),
+    end_com c2 -> checkpoint \notin O -> 
+( forall(l: loc ), ((getmap N1) l <> (getmap N1c) l) -> (l \in getfstwt W))
+-> all_diff_in_fw N1 V1 c1 N1c.
+
+(*Definition 5 in Technical Appendix*)
+Inductive current_init_pt: nvmem -> vmem -> command -> nvmem -> nvmem -> nvmem -> Prop:=
+  valid_mem: forall {N Ni0 N1 Nc0 Nend: nvmem}
+                  {V V1 Vend: vmem}
+                  {c crem: command}
+                  {W : the_write_stuff}
+                  {O: obseq}
+                  {w: warvars}
+                  (T: trace_cs (Ni0, V, c) (Nend, Vend, crem) O W),
+    crem = skip \/ (exists(w: warvars) (crem2: command), crem = ((incheckpoint w);;crem2)) ->
+    subseq (getdomain Nc0) (getdomain N1)
+    -> subset_nvm N Nc0
+                  -> (checkpoint \notin O) 
+                 -> (forall(l: loc),
+                      not((getmap N1) l = (getmap Nc0) l)
+                      -> (l \in (getfstwt W)) \/ (l \in (getdomain N)))
+                 -> current_init_pt N V c Ni0 N1 Nc0.
+
+(*Definition 4 in Technical Appendix*)
+Inductive same_pt: nvmem -> vmem -> command -> command -> nvmem -> nvmem -> Prop :=
+same_mem: forall {N0 N1 Ncomp N2: nvmem}
+                  {V0 V1 V2: vmem}
+                  {c0 c1 crem: command}
+                  {W1 W2: the_write_stuff}
+                  {O1 O2: obseq}
+                  (T1: trace_cs (N0, V0, c0) (N1, V1, c1) O1 W1)
+                  (T2: trace_cs (N1, V1, c1) (N2, V2, crem) O2 W2),
+    crem = skip \/ (exists(w: warvars) (crem2: command), crem = ((incheckpoint w);;crem2)) ->
+                  subseq (getdomain Ncomp) (getdomain Ncomp) 
+                  -> (checkpoint \notin O1)
+                  -> (checkpoint \notin O2) 
+                 -> (forall(l: loc),
+                      not((getmap N1) l = (getmap Ncomp) l)
+                      -> ((l \in (getwt W2)) /\ (l \in (getfstwt (append_write W1 W2))) /\ not (l \in (getwt W1))))
+                  -> same_pt N0 V0 c0 c1 N1 Ncomp.
+
+(*Definition 6 in Technical Appendix*)
+Inductive same_config: nvmem -> iconf -> context -> Prop :=
+  SameConfig: forall(Nstart N0 N1 N2: nvmem)
+                (V0 V: vmem)
+                (c0 c: command),
+    subset_nvm N0 Nstart ->
+    same_pt Nstart V0 c0 c N1 N2 ->
+    same_config Nstart ((N0, V0, c0), N1, V, c) (N2, V, c).
+
+(*helper lemmas about all_diff_in_fw*)
+
+  Lemma adifw_adif {N V c N1}:
+    all_diff_in_fw N V c N1 ->
+    all_diff_in_fww N V c N1.
+    intros Hdiff. inversion Hdiff. subst.
+    econstructor; try apply T; try assumption. Qed.
+
+
+ Lemma agreeonread: forall{N Nend N2: nvmem} {V Vend: vmem}
+                        {c c1: command}
+                   {O : obseq} {W: the_write_stuff},
+  all_diff_in_fw N V c N2 ->
+             cceval_w (N, V, c) O (Nend, Vend, c1) W ->
+             ( forall(z: loc), z \in (getrd W) -> (getmap N) z = (getmap N2) z).
+   intros. apply adifw_adif in H. eapply agreeonread_w_l; try apply H; try apply H0; try assumption. Qed.
+
+ Lemma add_skip_ins {N1 V l N2}: all_diff_in_fw N1 V (Ins l) N2 ->
+                                 all_diff_in_fw N1 V (l;; skip) N2.
+   intros Hdiff. inversion Hdiff; subst.
+   inversion T; subst.
+   - destruct H as [one | two]. inversion one. subst.
+     econstructor.
+     eapply CsTrace_Single. eapply Skip. by left. by []. assumption. destruct two as [crem [w contra] ]. discriminate contra.
+     move: (cceval_skip H2) => one. subst.
+     econstructor. eapply CsTrace_Single.
+     eapply Seq. intros w contra. subst. inversion H2.
+     intros contra. subst. inversion H2. apply H2. by left.
+     assumption. assumption.
+     destruct Cmid as [ [nm vm] cm].
+     move: (cceval_skip H4) => eq. subst.
+     econstructor. eapply CsTrace_Single.
+     eapply Seq. intros w contra. subst. inversion H4.
+     intros contra. subst. inversion H4.
+     apply H4. by left.
+     rewrite mem_cat in H0. move/ norP: H0 => [Ho1 Ho2].
+     assumption.
+     suffices: W2 = emptysets. move => eq. subst.
+     rewrite append_write_empty in H1.
+     assumption.
+     move: (trace_skip H2) => Heq. subst. by move/empty_trace_cs1: H2 => [one two].
+ Qed.
+
+ Lemma adif_cceval {N1 N2 V c Nend Vend O1 W cend}:
+  all_diff_in_fw N1 V c N2 ->
+  cceval_w (N1, V, c) O1 (Nend, Vend, cend) W ->
+  end_com cend ->
+    forall(l: loc ), ((getmap N1) l <> (getmap N2) l) -> (l \in getfstwt W).
+  intros. move: l H2. inversion H; subst.
+  destruct (O == [::]) eqn: Hbool; move/ eqP: Hbool => Hnil. subst.
+  apply empty_trace_cs1 in T. destruct T as [one two]. inversion one. subst.
+  intros l contra. apply (H4 l) in contra.
+  rewrite in_nil in contra. discriminate contra.
+  move: (single_step_alls T Hnil H0). => [Wrest [Orest [ Trest [Hsub Hw] ] ] ].
+  suffices: checkpoint \notin Orest. move => Hrest.
+  move: (same_endcom_help Trest Hrest H1 H2) => one. subst.
+  move/ empty_trace_cs: Trest => [one [two [three four] ] ]. subst.
+ by rewrite append_write_empty in H4.
+ apply/negP. intros contra.
+ exfalso.
+ rewrite Hsub in H3.
+ move/ negP : H3. apply. rewrite mem_cat. apply/orP.
+by right.
+ Qed.
+
+
+(*if adif holds at the end of a checkpointed segment, then the related memories
+ must be equal*)
+Lemma trace_converge {N V cend Nc} :
+  all_diff_in_fw N V cend Nc ->
+  end_com cend ->
+  N = Nc.
+  intros Hdiff Hend. apply nvmem_eq.
+  inversion Hdiff. subst.
+  suffices: O = [::]. move => Heq. subst.
+  move/ empty_trace_cs1 : T => [one [two three] ]. subst.
+  apply/ eqP /negPn /negP. intros contra.
+  move/ eqP : contra => contra.
+  apply (H1 three) in contra. rewrite in_nil in contra. discriminate contra.
+  move: (same_endcom_help T H0 Hend H) => one. subst.
+    by move/ empty_trace_cs : T => [one [two three] ].
+    Qed.
+
+Lemma trace_converge_minus1 {N V N' Nmid Vmid Nmid'
+                            O W} {l: instruction}:
+  all_diff_in_fw N V l N' ->
+  cceval_w (N, V, Ins l) O (Nmid, Vmid, Ins skip) W ->
+  cceval_w (N', V, Ins l) O (Nmid', Vmid, Ins skip) W ->
+  Nmid = Nmid'.
+   intros. apply adifw_adif in H.
+   eapply trace_converge_minus1w; try apply H; try apply H0; try assumption. Qed.
+
+  Lemma two_bc {Ni Ni1 V V1 l c1 crem Nc O W} : all_diff_in_fw Ni V (l;;crem) Nc ->
+                              cceval_w (Ni, V, Ins l) O (Ni1, V1, c1) W ->
+                              exists(Nc1: nvmem), (cceval_w (Nc, V, Ins l) O (Nc1, V1, c1) W /\
+                                              forall(l: loc), l \in (getwt W) -> ((getmap Ni1) l = (getmap Nc1) l)).
+      intros.
+      apply adifw_adif in H.
+      eapply two_bcw; try apply H; try assumption. Qed.
+
+  (*all_diff_in_fw preserved under single step continuous evaluation*)
+Lemma two {Ni Ni1 V V1 c c1 Nc O W} : all_diff_in_fw Ni V c Nc ->
+                              cceval_w (Ni, V, c) O (Ni1, V1, c1) W ->
+                              exists(Nc1: nvmem), (cceval_w (Nc, V, c) O (Nc1, V1, c1) W /\
+                                              (forall(l: loc), l \in (getwt W) -> ((getmap Ni1) l = (getmap Nc1) l))
+
+                                             /\
+                                             (checkpoint \notin O -> all_diff_in_fw Ni1 V1 c1 Nc1)
+                                             ).
+  intros.
+  induction c.
+  - move: (two_bc (add_skip_ins H) H0). => [Nc1 [Hcceval Hl] ].
+    exists Nc1. repeat (split; try assumption).
+    move: (cceval_skip Hcceval) => Heq. subst.
+    pose proof (trace_converge_minus1 H H0 Hcceval). subst. intros.
+    econstructor; try reflexivity.
+    apply (CsTrace_Empty (Nc1, V1, Ins skip)). by left.
+      by rewrite in_nil.
+      move => l0 contra. exfalso. by apply contra.
+   - inversion H0; subst.
+     +
+       assert (end_com (incheckpoint w;; c1)) as Hcp.
+       right. by exists c1 w.
+       move: (trace_converge H Hcp) => one. subst.
+       exists Nc. repeat split. apply CheckPoint; try assumption.
+       move/ negP => contra. exfalso. by apply contra.
+     + exists Nc. repeat split. apply Skip. move => l contra.
+       rewrite in_nil in contra. by exfalso. intros.
+       inversion H; subst.
+       suffices: O <> [::]. intros Ho.
+       move: (single_step_alls T Ho H0). => [Wrest [Orest
+                                                     [Trest
+                                [Hsubseq Hwrite] ] ] ].
+       econstructor; try apply Trest; try assumption.
+       apply/negP. intros contra.
+       apply/negP / negPn: H3.
+ rewrite Hsubseq.
+rewrite mem_cat. apply/orP.
+by right.
+       rewrite append_write_empty_l in Hwrite. by rewrite - Hwrite.
+       intros contra. subst.
+       move: (empty_trace_cs1 T) => [Eq1 Eq2].
+       inversion Eq1. subst. inversion H2.
+       inversion H5.
+       move : H5 => [crem [w contra] ]. inversion contra.
+     + move: (two_bc H H12) => [Nc1 [Hsmall Hdone] ]. exists Nc1. repeat split; try assumption.
+       apply Seq; try assumption.
+       inversion H; subst.
+       suffices: O0 <> [::]. intros Ho.
+       move: (single_step_alls T Ho H0). => [Wrest [Orest
+                                                     [Trest
+                                [Hsubseq Hwrite] ] ] ].
+       econstructor; try apply Trest; try assumption.
+       apply/negP. intros contra.
+       apply/negP / negPn: H2.
+ rewrite Hsubseq.
+rewrite mem_cat. apply/orP.
+by right.
+       intros l0 Hl0. remember Hl0 as Hneq.
+           clear HeqHneq.
+           suffices: getmap Ni1 l0 <> getmap Nc1 l0 -> l0 \notin getwt W.
+           intros Hdonec. apply Hdonec in Hl0.
+           suffices: (l0 \in getfstwt W0).
+           intros Hfw.
+           subst. move/ fw_split : Hfw => [one | two].
+           apply (in_subseq (fw_subst_wt_c H12)) in one.
+           exfalso. move/ negP : Hl0. by apply.
+             by move: two => [whatever done].
+             apply H3.
+             move: (update_one_contra l0 H12 Hl0) => Heq1.
+             move: (update_one_contra l0 Hsmall Hl0) => Heq2.
+             by rewrite Heq1 Heq2.
+             clear Hneq. intros Hneq. apply/negP. intros contra.
+             apply Hneq. by apply Hdone.
+       intros contra. subst.
+       move: (empty_trace_cs1 T) => [Eq1 Eq2].
+       inversion Eq1. subst. inversion H1.
+       inversion H4.
+       move : H4 => [crem [w contra] ]. inversion contra.
+       by apply (H10 w).
+     + inversion H0; subst; exists Nc; repeat split. apply If_T.
+       move: (agreeonread H H0) => agr.
+       apply (agr_imp_age H11); try assumption.
+       move => l contra.
+       rewrite in_nil in contra. by exfalso.
+       intros.
+       inversion H. subst. suffices: O <> [::]. intros Ho.
+       move: (single_step_alls T Ho H0). => [Wrest [Orest
+                                                     [Trest
+                                [Hsubseq Hwrite] ] ] ].
+       econstructor; try apply Trest; try assumption.
+       apply/negP.
+       move => contra. rewrite Hsubseq mem_cat in H3.
+       move/ norP : H3 => [one two].
+       move/negP: two.
+         by apply.
+         destruct W as [ [w1 w2 ] w3].
+         destruct Wrest as [ [wr1 wr2] wr3]. inversion Hwrite.
+         rewrite cats0 in H8.
+         intros l Hneq. apply H4 in Hneq. subst. simpl in Hneq.
+         simpl. rewrite mem_filter in Hneq.
+         by move/ andP : Hneq => [one two].
+       intros contra. subst. move: (empty_trace_cs1 T) => [Eq1 Eq2].
+       inversion Eq1. subst. inversion H2.
+       inversion H5.
+       move : H5 => [crem [w contra] ]. inversion contra.
+       apply If_F.
+       move: (agreeonread H H0) => agr.
+       apply (agr_imp_age H11); try assumption. move => l contra.
+       rewrite in_nil in contra. by exfalso.
+       intros.
+       inversion H. subst. suffices: O <> [::]. intros Ho.
+       move: (single_step_alls T Ho H0). => [Wrest [Orest
+                                                     [Trest
+                                [Hsubseq Hwrite] ] ] ].
+       econstructor; try apply Trest; try assumption.
+       apply/negP.
+       move => contra. rewrite Hsubseq mem_cat in H3.
+       move/ norP : H3 => [one two].
+       move/negP: two.
+         by apply.
+         destruct W as [ [w1 w2 ] w3].
+         destruct Wrest as [ [wr1 wr2] wr3]. inversion Hwrite.
+         rewrite cats0 in H8.
+         intros l Hneq. apply H4 in Hneq. subst. simpl in Hneq.
+         simpl. rewrite mem_filter in Hneq.
+         by move/ andP : Hneq => [one two].
+       intros contra. subst. move: (empty_trace_cs1 T) => [Eq1 Eq2].
+       inversion Eq1. subst. inversion H2.
+       inversion H5.
+       move : H5 => [crem [w contra] ]. inversion contra.
+Qed.
+
+Lemma two_p_five {Ni Ni1 V V1 c c1 Nc O W} : all_diff_in_fw Ni V c Nc ->
+                                             cceval_w (Ni, V, c) O (Ni1, V1, c1) W ->
+                                             checkpoint \notin O ->
+                              exists(Nc1: nvmem), (cceval_w (Nc, V, c) O (Nc1, V1, c1) W /\
+                              all_diff_in_fw Ni1 V1 c1 Nc1).
+  intros.
+  move: (two H H0) => [Nc1 [Hcceval [Hl Hdone] ] ]. exists Nc1. split; try assumption. by apply Hdone.
+Qed.
+
+(*if two memories are related and there is a continuous trace starting from one and ending
+at the end of a checkpointed segment, there is an identical continuous trace starting from the other *)
+Lemma adif_works {N1 N2 V c Nend Vend O1 W1 cend}:
+  all_diff_in_fw N1 V c N2 ->
+  trace_cs (N1, V, c) (Nend, Vend, cend) O1 W1 ->
+  end_com cend -> checkpoint \notin O1 ->
+  trace_cs (N2, V, c) (Nend, Vend, cend) O1 W1.
+  intros. move: N2 H.
+  dependent induction H0; intros.
+  + move: (trace_converge H H1) => Heq. subst.
+    apply (CsTrace_Empty (N2, Vend, cend)).
+  + move: (adif_cceval H0 H H1) => Hl.
+    move: (two H0 H) => [Nend1 [Hcceval Hl2] ].
+    suffices: Nend = Nend1.
+    intros. subst. by apply CsTrace_Single.
+    apply nvmem_eq.  intros l.
+    destruct (l \in getwt(W)) eqn: Hbool.
+       - apply Hl2. apply Hbool.
+       -
+         suffices: getmap N1 l = getmap N2 l.
+         intros Heq.
+         move: (update_one_c l H) => Himp1.
+         apply contra in Himp1.
+         move: (update_one_c l Hcceval) => Himp2.
+         apply contra in Himp2.
+         move /negPn/ eqP: Himp1.
+         move /negPn/ eqP: Himp2.
+         intros. rewrite - Himp1.
+           by rewrite - Himp2.
+           by move/ negbT: Hbool.
+             by move/ negbT: Hbool.
+          apply/ eqP.
+          destruct (getmap N1 l == getmap N2 l) eqn: Hbool1.
+          auto.
+          move/ eqP : Hbool1.
+          move/Hl => Hcontra.
+          move: (fw_subst_wt_c H) => Hsub.
+          apply (in_subseq Hsub) in Hcontra.
+            by rewrite Hbool in Hcontra.
+         + destruct Cmid as [ [Ni1 V1] c1].
+           assert (checkpoint \notin O1) as Hcp1.
+           apply/negP. intros contra.
+           apply/negP/ negPn: H3.
+           by apply in_app_l.
+           move: (two_p_five H4 H1 Hcp1) => [Nmid [Hccevalmid Hdiff] ].
+           eapply CsTrace_Cons.
+           eapply IHtrace_cs; try reflexivity; 
+             try assumption; try apply Hdiff.
+           apply/negP. intros contra.
+           apply/negP/ negPn: H3.
+           by apply in_app_r. assumption. assumption.
+Qed.
+
+(*ramping up to the final proof*)
+Lemma adif_refl {N V c c1 Nend Vend O W}:
+  trace_cs (N, V, c) (Nend, Vend, c1) O W ->
+  end_com c1 ->
+  checkpoint \notin O ->
+        all_diff_in_fw N V c N.
+  intros. econstructor; try apply H; try assumption; try by [].
+  Qed.
+
+   Lemma adif_sym {N1 V1 c1 Nc1}:
+  all_diff_in_fw N1 V1 c1 Nc1 ->
+  all_diff_in_fw Nc1 V1 c1 N1.
+  intros Hdiff. inversion Hdiff. subst.
+  move: (adif_works Hdiff T H H0) => Tdone.
+  econstructor; try apply Tdone; try assumption.
+ intros z Hz. 
+ apply not_eq_sym in Hz. by apply H1.
+Qed.
+
+Lemma adif_trans {Nc0 V1 c1 Nc1 Nc2}:
+  all_diff_in_fw Nc0 V1 c1 Nc1 ->
+  all_diff_in_fw Nc1 V1 c1 Nc2 ->
+  all_diff_in_fw Nc0 V1 c1 Nc2.
+  intros Hd1 Hd2. inversion Hd1. inversion Hd2. subst.
+  move: (adif_works Hd1 T H H0) => Td1.
+  move: (same_endcom Td1 T0 H H6 H0 H7) => Heq. subst.
+  move: (determinism Td1 T0) => [one two]. subst.
+  econstructor; try apply T; try assumption. 
+  intros l Hneq.
+  destruct (getmap Nc0 l == getmap Nc1 l) eqn:Hbool; move/ eqP : Hbool => Heq. rewrite Heq in Hneq. by apply H8 in Hneq.
+  by apply H1 in Heq.
+Qed.
+
+
+Lemma three_bc1 {Ni Ni1 V V1 c c1 Nc O W} :
+  all_diff_in_fw Ni V c Nc ->
+  cceval_w ( Ni, V, c) O (Ni1, V1, c1) W ->
+    checkpoint \notin O ->
+  ( exists(Nc1: nvmem), cceval_w (Nc, V, c) O (Nc1, V1, c1) W /\
+                   all_diff_in_fw Ni1 V1 c1 Nc1).
+intros. move: (two H H0) => [Nc1 [Hcceval Heq] ]. exists Nc1.
+    split. assumption. 
+    inversion H. subst. 
+    assert (O0 <> [::]) as Ho0.
+-
+  intros Heq1. subst.
+  move/empty_trace_cs1 : T => [ [contra10 [contra11 contra12] ] contra2]. subst. case H2 as [Hskip | [crem [w Hcp] ] ]; subst.
+    inversion Hcceval. move/negP : H1. apply.
+    apply (observe_checkpt_s Hcceval).
+         move: (single_step_alls T Ho0 H0) => [W1 [O1 [T1 [Hsub Hw ] ] ] ].
+         econstructor; try apply T1; try assumption.
+         apply/ negP => contra.
+         move/ negP : H3. apply.
+ rewrite Hsub.
+rewrite mem_cat. apply/orP.
+by right.
+         move => l Hl.
+         destruct ((getmap Ni l) == (getmap Nc l)) eqn: Hcase;
+           move/eqP: Hcase => Hcase.
+         move: (update_onec H0 Hcceval Hcase Hl) => Hw1.
+         apply Heq in Hw1. exfalso. by apply Hl.
+         apply H4 in Hcase. subst. move/fw_split : Hcase => [Hc1 | Hc2].
+         move : (in_subseq (fw_subst_wt_c H0) Hc1) => contra.
+         apply Heq in contra.
+         exfalso. by apply Hl. by destruct Hc2.
+Qed.
+
+(*if two memories are related and there is a continuous trace starting from one, there
+ is a continuous trace starting from the other with identical observations*)
+  Lemma three_bc  {Ni Ni1 V V1 c c1 Nc O W} :
+  all_diff_in_fw Ni V c Nc ->
+  trace_cs (Ni, V, c) (Ni1, V1, c1) O W ->
+  checkpoint \notin O ->
+  ( exists(Nc1: nvmem), trace_cs (Nc, V, c) (Nc1, V1, c1) O W /\
+                   all_diff_in_fw Ni1 V1 c1 Nc1).
+Proof. intros. move: Nc H. dependent induction H0; intros.
+    (*empty trace case*)
+  - exists Nc; split; auto; constructor.
+    (*cceval case*)
+  -  move: (three_bc1 H0 H H1) => [Nc1 [Hcceval Hdiff] ].
+     exists Nc1. split; try assumption. apply (CsTrace_Single Hcceval).
+  - (*inductive cs case*)
+    destruct Cmid as [ [Nmid Vmid] cmid]. Check three_bc1.
+    rewrite mem_cat in H2. move/norP : H2 => [H21 H22].
+    move: (three_bc1 H3 H1 H21) => [Ncmid [Tmid Hmid] ].
+    suffices: exists Nc1,
+               trace_cs (Ncmid, Vmid, cmid) (Nc1, V1, c1) O2 W2 /\
+               all_diff_in_fw Ni1 V1 c1 Nc1.
+  - move => [ Nc1 [Tmid2end Hmid2end] ]. exists Nc1. split; try assumption.
+    eapply CsTrace_Cons; try apply Tmid2end; try assumption.
+    eapply IHtrace_cs; try reflexivity; try assumption.
+ Qed.
+
+
+(*if two memories are related and there is an intermittent trace starting from one which does
+not cross a checkpoint boundary, there is a continuous trace starting from the other
+with identical observations (only unbroken by reboots).
+further, the relation is preserved from starting memories to ending memories,
+ and given that the intermittent ending memory can proceed continuously to the end of
+ a segment, the continuous ending memory can do the same, with related observations*)
+Lemma threeIS1 {N0 Ni Ni1 Nend V V1 Vend c c1 Nc O W Oend Wend cend}:
+  all_diff_in_fw Ni V c Nc -> 
+  trace_i1 ((N0, V, c), Ni, V, c) ((N0, V, c), Ni1, V1, c1) O W ->
+  WARok (getdomain N0) [::] [::] c ->
+  subset_nvm N0 Ni ->
+  checkpoint \notin O ->
+  trace_cs (Ni1, V1, c1) (Nend, Vend, cend) Oend Wend ->
+  end_com cend -> checkpoint \notin Oend ->
+  (exists(Oc Oendc: obseq) (Nc1: nvmem) (Wc Wendc: the_write_stuff),
+      trace_cs (Nc, V, c) (Nc1, V1, c1) Oc Wc /\
+      all_diff_in_fw Ni1 V1 c1 Nc1 /\ (O ++ Oend <=m Oc ++ Oendc)
+     /\ trace_cs (Nc1, V1, c1) (Nend, Vend, cend) Oendc Wendc
+  ).
+Proof. intros. move: Nc H H3.
+       dependent induction H0; intros.
+  + move: (three_bc H3 H H0) => [ Nc1 [Tdone Hdone] ].
+ exists O Oend Nc1 W Wend. repeat split; try assumption.
+    apply RB_Base; try (rewrite mem_cat; apply/ norP; split);
+    try assumption.
+    apply (neg_observe_rb H).
+    apply (neg_observe_rb H4).
+      apply (adif_works Hdone H4); try assumption.
+  + assert (all_diff_in_fw Ni V c (N0 U! Nmid)) as Hdiffrb.
+    - inversion H8. subst.  econstructor; try apply T; try assumption.
+   move => l. move/eqP/update_diff => [ [diff11 diff12] | [diff21 diff22] ]. case diff11. apply (H4 l diff12).
+   move: (update H (not_eq_sym diff21)) => Hdiff.
+   move: (wts_cped_sv H H3 H1 diff22 Hdiff)  => [good | bad].
+   rewrite/remove filter_predT in good.
+   apply (fw_gets_bigger H H1 T H10 good).
+   rewrite in_nil in bad. by discriminate bad.
+   suffices:
+               exists Oc Oendc Nc1 Wc Wendc,
+  trace_cs (Nc, V, c) (Nc1, V1, c1) Oc Wc /\
+  all_diff_in_fw Ni1 V1 c1 Nc1 /\
+  (O2 ++ Oend <=m Oc ++ Oendc) /\
+  trace_cs (Nc1, V1, c1) (Nend, Vend, cend) Oendc Wendc.
+   intros [Oc [Oendc [Nc1 [Wc [Wendc
+                                 [ass1
+                                    [ass2
+                                       [ass3 ass4] ] ] ] ] ] ] ].
+   exists Oc Oendc Nc1 Wc Wendc.
+   repeat split; try assumption.
+    assert (checkpoint \notin Oc ++ Oendc).
+    apply no_CP_in_seq in ass3.
+    by move: ass3 => [Ha1 Ha2].
+   rewrite- catA.
+   rewrite - catA.
+   apply RB_Ind; try assumption.
+   apply (neg_observe_rb H).
+   rewrite mem_cat; apply/ norP; split.
+    apply (neg_observe_rb ass1).
+    apply (neg_observe_rb ass4).
+    rewrite mem_cat.
+    apply/ norP.
+    split; assumption.
+      move: (three_bc H8 H H1) => [Nc3 [threetrace whatever] ].
+      move: (append_c ass1 ass4) => bigtrace.
+      apply (ctrace_det_obs threetrace H1 bigtrace); try assumption.
+   eapply IHtrace_i1; try reflexivity; try assumption.
+   apply sub_update. apply (adif_trans (adif_sym Hdiffrb) H8).
+
+  + repeat rewrite mem_cat in H3. move/norP: H3 => [Hb H3].
+        move/norP: H3 => [contra Hb1]. by case/negP : contra. 
+Qed.
+
+
+
+(*the same as threeIS1, only the intermittent trace can cross arbitrary checkpoint boundaries.
+ the final result follows pretty quickly from this; one need only apply three with (the continuous trace ending
+ at cend) equal to the empty trace*)
+Lemma three {N0 N01 V01 c01 Ni Ni1 Nend V V1 Vend c c1 Nc O W Oend Wend cend}:
+  all_diff_in_fw Ni V c Nc ->
+  trace_i1 ((N0, V, c), Ni, V, c) ((N01, V01, c01), Ni1, V1, c1) O W ->
+  WARok (getdomain N0) [::] [::] c ->
+  subset_nvm N0 Ni -> 
+  trace_cs (Ni1, V1, c1) (Nend, Vend, cend) Oend Wend ->
+  end_com cend -> checkpoint \notin Oend ->
+  (exists(Oc Oendc: obseq) (Nc1: nvmem) (Wc Wendc: the_write_stuff) ,
+      trace_cs (Nc, V, c) (Nc1, V1, c1) Oc Wc /\
+      all_diff_in_fw Ni1 V1 c1 Nc1 /\ (O ++ Oend <=f (Oc ++ Oendc)) /\
+      trace_cs (Nc1, V1, c1) (Nend, Vend, cend) Oendc Wendc
+  ).
+Proof.
+  intros. move: Nc H H3. dependent induction H0; intros.
+  + move: (three_bc H3 H H0) => [ Nc1 [Tdone Hdone] ].
+    exists O Oend Nc1 W Wend. repeat split; try assumption.
+    apply CP_Base. apply RB_Base; try (rewrite mem_cat; apply/ norP; split);
+    try assumption.
+    apply (neg_observe_rb H).
+    apply (neg_observe_rb H6).
+    apply (adif_works Hdone H6); try assumption.
+  + 
+    move: (iTrace_RB H H0 H1 H2) => bigtrace.
+    assert (checkpoint \notin O1 ++ [:: reboot] ++ O2) as Hcp.
+    rewrite mem_cat. apply/ norP. split; try assumption.
+move: (threeIS1 H7 bigtrace H3 H4 Hcp H8 H5 H6) =>
+[Oc
+   [Oendc
+      [Nc1
+         [Wc [
+              Wendc
+               [ ass1 [
+                     ass2
+                       [ass3 ass4]
+                   ]
+               ]
+            ]
+         ]
+      ]
+   ]
+].
+exists Oc Oendc Nc1 Wc Wendc. repeat split; try assumption.
+repeat rewrite - catA.
+apply CP_Base.
+by repeat rewrite - catA in ass3.
+  +
+        remember ((incheckpoint w);;crem) as ccp.
+       assert (end_com ccp) as Hend. unfold end_com. right.
+       subst.
+         by exists crem w.
+        suffices: (exists Oc Oendc Nc1 Wc
+                 Wendc Nc1end Vc1end cend,
+                 trace_cs (Nc, V, c)
+                          (Nc1, Vmid, ccp) Oc Wc /\
+                 all_diff_in_fw Nmid Vmid ccp Nc1 /\
+                 (O1 <=m Oc) /\
+                 trace_cs (Nc1, Vmid, crem)
+                   (Nc1end, Vc1end, cend) Oendc
+                   Wendc /\ checkpoint \notin Oendc /\ end_com cend
+                  ).
+    - move => [Oc1 [Oendc1 [Nc1 [Wc1 [Wendc1 [ Nc1end [ Vc1end
+            [ ccend [H11 [H12 [Ho1 [H13 [H14 H15] ] ] ] ] ] ] ] ] ] ] ] ]. subst.
+      move: (trace_converge H12 Hend) => Heq. subst.
+      assert (WARok (getdomain
+                       (restrict Nc1 w Hw)) [::] [::] crem) as Hwarok2.
+      destruct Nc1 as [mc1 dc1 Hnc1]. rewrite/getdomain. simpl.
+      apply (warok_cp H1 H11). 
+        remember ((incheckpoint w);;crem) as ccp.
+      suffices: (
+                 exists Oc2 Oendc2 Nc2 Wc2 Wendc2,
+                   trace_cs (Nc1, Vmid, crem)
+                            (Nc2, V1, c1) Oc2 Wc2 /\
+                   all_diff_in_fw Ni1 V1 c1 Nc2 /\
+                   (O2 ++ Oend <=f Oc2 ++ Oendc2) /\
+                 trace_cs (Nc2, V1, c1) 
+                   (Nend, Vend, cend) Oendc2 Wendc2
+                ).
+      move => [Oc2 [Oendc2 [Nc2 [Wc2 [Wendc2 [H21 [H22 [Ho2 H23] ] ] ] ] ] ] ].
+     - subst. move: (append_cps H11 H21 Hw) => T1.
+      exists (Oc1 ++ [::checkpoint] ++ Oc2) Oendc2 Nc2 (append_write Wc1 Wc2) Wendc2.
+      repeat split; try assumption.
+      repeat rewrite - catA. apply CP_IND; try assumption.
+      - eapply IHtrace_i1_2;try reflexivity; try assumption;
+        try apply sub_restrict.
+        apply (adif_refl H13 H15 H14).
+       move: (trace_append_ic H0_0 H3 H5) => Tendi.
+              assert ( checkpoint \notin [::]) as Hcp.
+              by rewrite in_nil.
+       move: (threeIS1 H0 H0_ H1 H2 H
+                       (CsTrace_Empty
+                          (Nmid, Vmid, ccp )) Hend Hcp).
+       => [Oc [Oendc [Nc1 [Wc [ Wendc500 [T1 [Hdiff [Hm Tempty] ] ] ] ] ] ] ].
+       subst.
+       move: (trace_converge Hdiff) => Hsamemem. subst.
+       move/ empty_trace_cs : Tempty => [Heq
+                                          blah ].
+       subst.
+       move: (exist_endcom Tendi H4) => [Oendc0 [Wendc0 [Nc1end0 [Vc1end
+                                                           [cend0 [Tend [Hendcom Hoendc] ] ] ] ] ] ].
+      apply trace_converge in Hdiff. subst.
+      assert (WARok (getdomain
+                       (restrict Nc1 w Hw)) [::] [::] crem) as Hwarok2.
+      destruct Nc1 as [mc1 dc1 Hnc1]. rewrite/getdomain. simpl.
+      subst.
+      move: (same_comi H1 H2 H0_ H) => [Nend1 [Oc1 [Wc1 [Tc1 Hoc1] ] ] ].
+      apply (warok_cp H1 Tc1).
+       subst.
+      move: (same_comi Hwarok2 (sub_restrict Nc1 w Hw) Tend Hoendc).
+      =>
+      [Nc1end [Oendc [Wendc [Tendc Hcpoendc] ] ] ].                                                            
+       exists Oc Oendc Nc1 Wc Wendc Nc1end. exists Vc1end cend0. subst.
+       repeat split; try assumption. 
+       econstructor; try eapply CsTrace_Empty; auto.
+       by repeat rewrite cats0 in Hm. assumption.
+Qed.
+
+(*proof that definition 1 from 'Towards a Formal Foundation' holds for
+ any intermittent trace which satisfies the WARok relation*)
+Theorem One {N0 V c N01 V01 c01 N Oi Nendi Vend Wi
+           }:
+      trace_i1 ((N0, V, c), N, V, c) ((N01, V01, c01), Nendi, Vend, Ins skip) Oi Wi ->
+subset_nvm N0 N -> 
+WARok (getdomain N0) [::] [::] c ->
+(exists (Oc: obseq) (Wc: the_write_stuff) , trace_cs (N, V, c) (Nendi, Vend, Ins skip) Oc Wc /\
+                                                     (Oi <=f Oc)).
+  intros.
+assert (end_com skip) as Hskip. by left.
+suffices: 
+  (exists(Oc Oendc: obseq) (Nendc: nvmem) (Wc Wendc: the_write_stuff),
+      trace_cs (N, V, c) (Nendc, Vend, Ins skip) Oc Wc /\
+ all_diff_in_fw Nendi Vend skip Nendc /\ trace_cs (Nendc, Vend, Ins skip)
+            (Nendc, Vend, Ins skip) Oendc Wendc
+  ).
+move => [Oc
+          [ Oendc [Nendc
+             [Wc
+                [Wendc
+                   [Tc
+                      [Hdiff Tend] ] ] ] ] ] ].
+exists Oc Wc. repeat skip; try assumption.
+suffices: all_diff_in_fw N V c N.
+move => Hdiff.
+move: (three Hdiff H H1 H0 (CsTrace_Empty (Nendi, Vend, (Ins skip))) Hskip
+      (notin checkpoint)).
+=> [Oc [Oendc [Nendc [Wc [ Wendc [T1 [Hdiffend [Hm Tempty] ] ] ] ] ] ] ].
+exists Oc Oendc Nendi Wc Wendc.
+move: (empty_trace_cs Tempty). => [Ho [Hn [Hv Hw] ] ]. subst.
+repeat split; try assumption.
+move: (exist_endcom H Hskip) => [Osmall
+                                  [Wsmall
+                                     [Nmid
+                                     [Vmid
+                                           [cmid
+                                              [Tsmall
+                                                 [Hend Hcp ]  ] ] ] ] ] ].
+move: (same_comi H1 H0 Tsmall Hcp) => [N2 [Osc [c2 [Tsc Hosc] ] ] ].
+econstructor; try apply Tsc; try assumption.
+  by intros.
+ Qed.
+
+
+
